@prefix ls: <http://labeling.i3mainz.hs-mainz.de/vocab#>.
@prefix owl: <http://www.w3.org/2002/07/owl#>.
@prefix rdfs: <http://www.w3.org/2000/01/rdf-schema#>.
@prefix rdf: <http://www.w3.org/1999/02/22-rdf-syntax-ns#>.
@prefix dcterms: <http://purl.org/dc/terms/>.
@prefix xsd: <http://www.w3.org/2001/XMLSchema#>.
@prefix skos: <http://www.w3.org/2004/02/skos/core#>.

# Ontology

ls: a owl:Ontology;
	rdfs:label "Labeling System Vocabulary"@en;
	dcterms:created "2016-07-20"^^xsd:date;
	dcterms:description "A RDF vocabulary describing the Labeling System ontology"@en;
	owl:versionInfo "Aldgate Edition";
	dcterms:creator "Florian Thiery M.Sc., mainzed";
	dcterms:licence <http://creativecommons.org/licenses/by/4.0/>;
	rdfs:seeAlso <http://labeling.i3mainz.hs-mainz.de/vocab/index.htm>.

# Classes

# Main Classes

ls:Agent a owl:Class;
	skos:definition <http://labeling.i3mainz.hs-mainz.de/ls-reference#MainClasses>;
	rdfs:label "Labeling System Agent"@en;
	rdfs:isDefinedBy <http://labeling.i3mainz.hs-mainz.de/vocab>.

ls:Label a owl:Class;
	skos:definition <http://labeling.i3mainz.hs-mainz.de/ls-reference#MainClasses>;
	rdfs:label "Labeling System Label"@en;
	rdfs:isDefinedBy <http://labeling.i3mainz.hs-mainz.de/vocab>.

ls:Revision a owl:Class;
	skos:definition <http://labeling.i3mainz.hs-mainz.de/ls-reference#MainClasses>;
	rdfs:label "Labeling System Revision"@en;
	rdfs:isDefinedBy <http://labeling.i3mainz.hs-mainz.de/vocab>.

ls:Vocabulary a owl:Class;
	skos:definition <http://labeling.i3mainz.hs-mainz.de/ls-reference#MainClasses>;
	rdfs:label "Labeling System Vocabulary"@en;
	rdfs:isDefinedBy <http://labeling.i3mainz.hs-mainz.de/vocab>.

# Release Type Classes

ls:ReleaseType a owl:Class;
	skos:definition <http://labeling.i3mainz.hs-mainz.de/ls-reference#ReleaseTypeClasses>;
	rdfs:label "release type"@en;
	rdfs:isDefinedBy <http://labeling.i3mainz.hs-mainz.de/vocab>.

ls:Public a owl:Class;
	rdfs:SubClassOf ls:ReleaseType;
	skos:definition <http://labeling.i3mainz.hs-mainz.de/ls-reference#ReleaseTypeClasses>;
	rdfs:label "public item"@en;
	rdfs:isDefinedBy <http://labeling.i3mainz.hs-mainz.de/vocab>.

ls:Draft a owl:Class;
	rdfs:SubClassOf ls:ReleaseType;
	skos:definition <http://labeling.i3mainz.hs-mainz.de/ls-reference#ReleaseTypeClasses>;
	rdfs:label "item in draft mode"@en;
	rdfs:isDefinedBy <http://labeling.i3mainz.hs-mainz.de/vocab>.

# Status Type Classes

ls:StatusType a owl:Class;
	skos:definition <http://labeling.i3mainz.hs-mainz.de/ls-reference#StatusTypeClasses>;
	rdfs:label "status type"@en;
	rdfs:isDefinedBy <http://labeling.i3mainz.hs-mainz.de/vocab>.

ls:Active a owl:Class;
	rdfs:SubClassOf ls:StatusType;
	skos:definition <http://labeling.i3mainz.hs-mainz.de/ls-reference#StatusTypeClasses>;
	rdfs:label "active item"@en;
	rdfs:isDefinedBy <http://labeling.i3mainz.hs-mainz.de/vocab>.

ls:Deleted a owl:Class;
	rdfs:SubClassOf ls:StatusType;
	skos:definition <http://labeling.i3mainz.hs-mainz.de/ls-reference#StatusTypeClasses>;
	rdfs:label "deleted item"@en;
	rdfs:isDefinedBy <http://labeling.i3mainz.hs-mainz.de/vocab>.

# Revision Type Classes

ls:RevisionType a owl:Class;
	skos:definition <http://labeling.i3mainz.hs-mainz.de/ls-reference#RevisionTypeClasses>;
	rdfs:label "Revision Type"@en;
	rdfs:isDefinedBy <http://labeling.i3mainz.hs-mainz.de/vocab>.

ls:CreateRevision a owl:Class;
	rdfs:SubClassOf ls:RevisionType;
	skos:definition <http://labeling.i3mainz.hs-mainz.de/ls-reference#RevisionTypeClasses>;
	rdfs:label "Revision Type to describe a create event"@en;
	rdfs:isDefinedBy <http://labeling.i3mainz.hs-mainz.de/vocab>.

ls:ModifyRevision a owl:Class;
	rdfs:SubClassOf ls:RevisionType;
	skos:definition <http://labeling.i3mainz.hs-mainz.de/ls-reference#RevisionTypeClasses>;
	rdfs:label "Revision Type to describe a modification event"@en;
	rdfs:isDefinedBy <http://labeling.i3mainz.hs-mainz.de/vocab>.

ls:DeleteRevision a owl:Class;
	rdfs:SubClassOf ls:RevisionType;
	skos:definition <http://labeling.i3mainz.hs-mainz.de/ls-reference#RevisionTypeClasses>;
	rdfs:label "Revision Type to describe a delete event"@en;
	rdfs:isDefinedBy <http://labeling.i3mainz.hs-mainz.de/vocab>.

ls:DescriptionRevision a owl:Class;
	rdfs:SubClassOf ls:ModifyRevision;
	skos:definition <http://labeling.i3mainz.hs-mainz.de/ls-reference#RevisionTypeClasses>;
	rdfs:label "Revision Type to describe a textural description modification event"@en;
	rdfs:isDefinedBy <http://labeling.i3mainz.hs-mainz.de/vocab>.

ls:LinkingRevision a owl:Class;
	rdfs:SubClassOf ls:ModifyRevision;
	skos:definition <http://labeling.i3mainz.hs-mainz.de/ls-reference#RevisionTypeClasses>;
	rdfs:label "Revision Type to describe a linking modification event"@en;
	rdfs:isDefinedBy <http://labeling.i3mainz.hs-mainz.de/vocab>.

ls:ShareRevision a owl:Class;
	rdfs:SubClassOf ls:ModifyRevision;
	skos:definition <http://labeling.i3mainz.hs-mainz.de/ls-reference#RevisionTypeClasses>;
	rdfs:label "Revision Type to describe a share modification event"@en;
	rdfs:isDefinedBy <http://labeling.i3mainz.hs-mainz.de/vocab>.

ls:SystemRevision a owl:Class;
	rdfs:SubClassOf ls:ModifyRevision;
	skos:definition <http://labeling.i3mainz.hs-mainz.de/ls-reference#RevisionTypeClasses>;
	rdfs:label "Revision Type to describe a internal modification event"@en;
	rdfs:isDefinedBy <http://labeling.i3mainz.hs-mainz.de/vocab>.

# Properties

# describing properties

ls:hasReleaseType a owl:ObjectProperty, rdf:Property;
	skos:definition <http://labeling.i3mainz.hs-mainz.de/ls-reference#DescribingProperties>;
	rdfs:label "has release type"@en;
	rdfs:domain ls:Vocabulary;
	rdfs:range ls:ReleaseType;
	rdfs:isDefinedBy <http://labeling.i3mainz.hs-mainz.de/vocab>.

ls:hasStatusType a owl:ObjectProperty, rdf:Property;
	skos:definition <http://labeling.i3mainz.hs-mainz.de/ls-reference#DescribingProperties>;
	rdfs:label "has status type"@en;
	rdfs:domain ls:Vocabulary, ls:Label;
	rdfs:range ls:StatusType;
	rdfs:isDefinedBy <http://labeling.i3mainz.hs-mainz.de/vocab>.

ls:preferredLabel a owl:ObjectProperty, rdf:Property;
	skos:definition <http://labeling.i3mainz.hs-mainz.de/ls-reference#DescribingProperties>;
	rdfs:label "has preffered label"@en;
	rdfs:domain ls:Label;
	rdfs:range xsd:string;
	rdfs:isDefinedBy <http://labeling.i3mainz.hs-mainz.de/vocab>.

ls:hasContext a owl:ObjectProperty, rdf:Property;
	skos:definition <http://labeling.i3mainz.hs-mainz.de/ls-reference#DescribingProperties>;
	rdfs:label "has context ID"@en;
	rdfs:domain ls:Label;
	rdfs:range xsd:string;
	rdfs:isDefinedBy <http://labeling.i3mainz.hs-mainz.de/vocab>.